WMM lemmas

src/example/WMM.v
@@ -34,6 +34,8 @@ Module WMem.
 
   Let ident := (Loc.t * Time.t)%type.
 
+  Definition view_to_local (vw: View.t): Local.t := Local.mk (TView.mk (fun _ => vw) vw vw) Memory.bot.
+
   Definition missed (m: Memory.t) (loc: Loc.t) (ts: Time.t): fmap ident :=
     fun '(loc', ts') =>
       if (Loc.eq_dec loc' loc)
@@ -47,13 +49,13 @@ Module WMem.
       else Flag.emp.
 
   Definition load_fun:
-    ktree (((@eventE ident) +' cE) +' sE t) (TView.t * Loc.t * Ordering.t) (TView.t * Const.t) :=
-    fun '(tvw0, loc, ord) =>
+    ktree (((@eventE ident) +' cE) +' sE t) (View.t * Loc.t * Ordering.t) (View.t * Const.t) :=
+    fun '(vw0, loc, ord) =>
       msc <- trigger (@Get _);;
       '(exist _ (lc1, val, to) _) <- trigger (Choose (sig (fun '(lc1, val, to) =>
                                                              exists released,
                                                                Local.read_step
-                                                                 (Local.mk tvw0 Memory.bot)
+                                                                 (view_to_local vw0)
                                                                  (msc.(memory))
                                                                  loc
                                                                  to
@@ -62,17 +64,17 @@ Module WMem.
                                                                  ord
                                                                  lc1)));;
       _ <- trigger (Fair (missed msc loc to));;
-      Ret (lc1.(Local.tview), val)
+      Ret (lc1.(Local.tview).(TView.cur), val)
   .
 
   Definition store_fun:
-    ktree (((@eventE ident) +' cE) +' sE t) (TView.t * Loc.t * Const.t * Ordering.t) (TView.t) :=
-    fun '(tvw0, loc, val, ord) =>
+    ktree (((@eventE ident) +' cE) +' sE t) (View.t * Loc.t * Const.t * Ordering.t) (View.t) :=
+    fun '(vw0, loc, val, ord) =>
       msc <- trigger (@Get _);;
       '(exist _ (lc1, to, sc1, mem1) _) <- trigger (Choose (sig (fun '(lc1, to, sc1, mem1) =>
                                                                    exists from released kind,
                                                                      Local.write_step
-                                                                       (Local.mk tvw0 Memory.bot)
+                                                                       (view_to_local vw0)
                                                                        (msc.(sc))
                                                                        (msc.(memory))
                                                                        loc
@@ -88,18 +90,18 @@ Module WMem.
                                                                        kind)));;
       _ <- trigger (Fair (missed msc loc to));;
       _ <- trigger (Put (mk mem1 sc1));;
-      Ret (lc1.(Local.tview))
+      Ret (lc1.(Local.tview).(TView.cur))
   .
 
   Definition faa_fun:
-    ktree (((@eventE ident) +' cE) +' sE t) (TView.t * Loc.t * Const.t * Ordering.t * Ordering.t) (TView.t * Const.t) :=
-    fun '(tvw0, loc, addendum, ordr, ordw) =>
+    ktree (((@eventE ident) +' cE) +' sE t) (View.t * Loc.t * Const.t * Ordering.t * Ordering.t) (View.t * Const.t) :=
+    fun '(vw0, loc, addendum, ordr, ordw) =>
       msc <- trigger (@Get _);;
       '(exist _ (lc2, to, val, sc1, mem1) _) <-
         trigger (Choose (sig (fun '(lc2, to, val, sc1, mem1) =>
                                 exists lc1 from releasedr releasedw kind,
                                   (Local.read_step
-                                     (Local.mk tvw0 Memory.bot)
+                                     (view_to_local vw0)
                                      (msc.(memory))
                                      loc
                                      from
@@ -124,7 +126,7 @@ Module WMem.
                                        kind))));;
       _ <- trigger (Fair (missed msc loc to));;
       _ <- trigger (Put (mk mem1 sc1));;
-      Ret (lc2.(Local.tview), val)
+      Ret (lc2.(Local.tview).(TView.cur), val)
   .
 
   Definition mod: Mod.t :=
@@ -163,18 +165,18 @@ Section MEMRA.
     OwnM (memory_resource_black m).
 
   (* normal points-to *)
-  Definition wpoints_to (l: Loc.t) (v: Const.t) (vw: TView.t): iProp :=
+  Definition wpoints_to (l: Loc.t) (v: Const.t) (vw: View.t): iProp :=
     ∃ c,
       (points_to l c)
         **
         (⌜exists from released,
               (<<GET: Cell.get (Cell.max_ts c) c = Some (from, Message.concrete v released)>>) /\
                 (<<DEFINED: v <> Const.undef>>) /\
-                (<<VIEW: View.le (View.singleton_ur l (Cell.max_ts c)) vw.(TView.cur) >>)⌝)
+                (<<VIEW: View.le (View.singleton_ur l (Cell.max_ts c)) vw >>)⌝)
   .
 
   Lemma wpoints_to_view_mon l v vw0 vw1
-        (LE: TView.le vw0 vw1)
+        (LE: View.le vw0 vw1)
     :
     (wpoints_to l v vw0)
       ⊢
@@ -182,7 +184,7 @@ Section MEMRA.
   Proof.
     unfold wpoints_to.
     iIntros "[% [OWN %]]". des. iExists _. iSplit; [iFrame|].
-    iPureIntro. esplits; eauto. etrans; eauto. eapply LE.
+    iPureIntro. esplits; eauto.
   Qed.
 
   Lemma wmemory_ra_get
@@ -240,25 +242,21 @@ Section MEMRA.
   Lemma wmemory_ra_load
         m l v0 v1 vw0 vw1
         ord lc1 to released
-        (READ: Local.read_step (Local.mk vw0 Memory.bot) m.(WMem.memory) l to v1 released ord lc1)
-        (VIEW: vw1 = lc1.(Local.tview))
+        (READ: Local.read_step (WMem.view_to_local vw0) m.(WMem.memory) l to v1 released ord lc1)
+        (VIEW: vw1 = lc1.(Local.tview).(TView.cur))
         (ORD: ord = Ordering.plain)
     :
     (wmemory_black m)
       -∗
       (wpoints_to l v0 vw0)
       -∗
-      ((wmemory_black m) ∗ (⌜(TView.le vw0 vw1) /\ (v0 = v1)⌝) ∗ #=>(wpoints_to l v0 vw1)).
+      ((wmemory_black m) ∗ (⌜(View.le vw0 vw1) /\ (v0 = v1)⌝) ∗ #=>(wpoints_to l v0 vw1)).
   Proof.
     iIntros "BLACK [% [WHITE %]]". des. subst.
     iPoseProof (wmemory_ra_get with "BLACK WHITE") as "%". subst.
     iSplitL "BLACK"; [auto|]. inv READ. ss. iSplit.
     { iPureIntro. split.
-      { econs; ss.
-        { i. reflexivity. }
-        { etrans; [|eapply View.join_l]. eapply View.join_l. }
-        { etrans; [|eapply View.join_l]. eapply View.join_l. }
-      }
+      { etrans; [|eapply View.join_l]. eapply View.join_l. }
       { assert (to = (Cell.max_ts (WMem.memory m l))).
         { eapply TimeFacts.antisym.
           { eapply Memory.max_ts_spec in GET0. des. clarify. }
@@ -283,8 +281,8 @@ Section MEMRA.
   Lemma wmemory_ra_store
         m0 l v0 vw0 m1 v1 vw1
         lc1 to sc1 mem1 ord from released kind
-        (WRITE: Local.write_step (Local.mk vw0 Memory.bot) m0.(WMem.sc) m0.(WMem.memory) l from to v1 None released ord lc1 sc1 mem1 kind)
-        (VIEW: vw1 = lc1.(Local.tview))
+        (WRITE: Local.write_step (WMem.view_to_local vw0) m0.(WMem.sc) m0.(WMem.memory) l from to v1 None released ord lc1 sc1 mem1 kind)
+        (VIEW: vw1 = lc1.(Local.tview).(TView.cur))
         (MEM: m1 = WMem.mk mem1 sc1)
         (ORD: ord = Ordering.plain)
         (DEFINED: v1 <> Const.undef)
@@ -293,7 +291,7 @@ Section MEMRA.
       -∗
       (wpoints_to l v0 vw0)
       -∗
-      ((⌜TView.le vw0 vw1⌝) ∗ #=>((wmemory_black m1) ∗ (wpoints_to l v1 vw1))).
+      ((⌜View.le vw0 vw1⌝) ∗ #=>((wmemory_black m1) ∗ (wpoints_to l v1 vw1))).
   Proof.
     iIntros "BLACK [% [WHITE %]]". des. subst.
     iPoseProof (wmemory_ra_get with "BLACK WHITE") as "%". subst.
@@ -307,27 +305,17 @@ Section MEMRA.
       { des; ss. eapply Memory.max_ts_spec in GET0. des.
         hexploit Memory.max_ts_spec.
         { eapply Memory.add_get0; eauto. }
-        i. des. rr in WRITABLE. inv WRITALBLE.
-
-
-        eapply Memory.max_ts_spec in
-
-
-eapply Memory.max_ts_spec in MAX0. des.
-        exfalso.
-
-        admit.
+        i. des. inv WRITABLE.
+        exfalso. eapply Time.lt_strorder. eapply TimeFacts.lt_le_lt.
+        { eapply TS. }
+        etrans; eauto.
+        etrans; eauto.
+        inv VIEW0. ss. specialize (RLX l).
+        unfold TimeMap.singleton in RLX. setoid_rewrite LocFun.add_spec_eq in RLX. auto.
       }
     }
     subst. iSplit.
-    { iPureIntro. econs; ss.
-      { i. des_ifs. erewrite LocFun.add_spec. des_ifs.
-        { eapply View.join_l. }
-        { reflexivity. }
-      }
-      { eapply View.join_l. }
-      { eapply View.join_l. }
-    }
+    { iPureIntro. eapply View.join_l. }
     iPoseProof (wmemory_ra_set with "BLACK WHITE") as "> [BLACK WHITE]".
     instantiate (1:=mem1 l). iModIntro. iSplitL "BLACK".
     { assert (EQ: mem1 = (LocFun.add l (mem1 l) (WMem.memory m0))).
@@ -341,128 +329,115 @@ eapply Memory.max_ts_spec in MAX0. des.
     { ss. eapply View.join_r. }
   Qed.
 
-rr.
-
-
-; auto.
-
-
-
-    iModIntro. iSplit; eauto.
-
-    assert (View.le (View.singleton_ur l (Cell.max_ts (mem1 l)))
-                    (TView.cur (TView.write_tview vw0 (WMem.sc m0) l to Ordering.plain))).
-    { subst. nss. etrans; [|eapply View.join_r]. subst. reflexivity. }
-
-      cut (TimeMap.le (TimeMap.singleton l (Cell.max_ts (mem1 l))) (TimeMap.singleton l to)).
-      { i. econs; ss. } subst. refle
-      eapply TimeMap.singleton_spec. unfold TimeMap.singleton.
-      setoid_rewrite LocFun.add_spec. des_ifs. inv WRITABLE.
-      hexploit Memory.max_ts_spec.
-      { eapply Memory.add_get1; eauto. }
-      i. des. erewrite Memory.add_o in GET0; eauto. des_ifs; ss.
-      { des; clarify. reflexivity. }
-      { des; ss. }eapply Memory.max_ts_spec in GET0. des; clarify.
-        etrans; eauto.
-
- des; s
-      }{
-
- in GET. des.
-
-
-      etrans; [|left; eauto]. inv VIEW0. ss. etrans; eauto.
-      unfold TimeMap.singleton.
-      setoid_rewrite LocFun.add_spec. des_ifs.
-      eapply Memory.max_ts_spec in GET. des.
-
-
-
-      admit.
-    }
-    { zadmi
-
-
-reflexvity.
-
-
-
-ss
-
-ss.
-
-
-     eauinv WR
-
-TView.le
-
-    iSplitL "BLACK"; [auto|]. inv READ. ss. iSplit.
-    { iPureIntro. split.
-      { econs; ss.
-        { i. reflexivity. }
-        { etrans; [|eapply View.join_l]. eapply View.join_l. }
-        { etrans; [|eapply View.join_l]. eapply View.join_l. }
-      }
-      { assert (to = (Cell.max_ts (WMem.memory m l))).
-        { eapply TimeFacts.antisym.
-          { eapply Memory.max_ts_spec in GET0. des. clarify. }
-          { inv READABLE. etrans; eauto.
-            inv VIEW0. ss. specialize (PLN0 l).
-            unfold TimeMap.singleton in PLN0.
-            setoid_rewrite LocFun.add_spec_eq in PLN0. auto.
-          }
-        }
-        subst. setoid_rewrite GET in GET0. clarify.
-        inv VAL; ss.
-        destruct v1, val'; ss. apply Z.eqb_eq in H0. subst. auto.
-      }
-    }
-    { iModIntro. iExists _. iFrame. iPureIntro. esplits; eauto.
-      ss. unfold View.singleton_ur_if. des_ifs.
-      etrans; eauto.
-      etrans; [|eapply View.join_l]. eapply View.join_l.
-    }
-  Qed.
-
-
-  Admitted.
-
-
   (* faa points-to *)
-  Definition wpoints_to_faa (l: Loc.t) (v: Const.t): iProp.
-  Admitted.
+  Definition wpoints_to_faa (l: Loc.t) (v: Const.t): iProp :=
+    ∃ c,
+      (points_to l c)
+        **
+        (⌜exists from released,
+              (<<GET: Cell.get (Cell.max_ts c) c = Some (from, Message.concrete v released)>>) /\
+                (<<FAA: forall to from msg (GET: Cell.get to c = Some (from, msg)),
+                    ((exists to' msg',
+                         (<<GET: Cell.get to' c = Some (to, msg')>>) /\ (<<TS: Time.lt to to'>>)) \/
+                       (<<TS: to = Cell.max_ts c>>))>>) /\
+                (<<DEFINED: v <> Const.undef>>)⌝)
+  .
 
   Lemma wmemory_ra_faa
         v msc
-        tvw0 loc addendum ordr ordw
+        vw0 loc addendum ordr ordw
         lc1 from releasedr releasedw kind
         lc2 to val sc1 mem1
-        (READ: Local.read_step (Local.mk tvw0 Memory.bot) (msc.(WMem.memory)) loc from val releasedr ordr lc1)
+        (READ: Local.read_step (WMem.view_to_local vw0) (msc.(WMem.memory)) loc from val releasedr ordr lc1)
         (WRITE: Local.write_step lc1 (msc.(WMem.sc)) (msc.(WMem.memory)) loc from to (Const.add val addendum) releasedr releasedw ordw lc2 sc1 mem1 kind)
         (ORDR: ordr = Ordering.plain)
         (ORDW: ordw = Ordering.acqrel)
+        (DEFINED: addendum <> Const.undef)
     :
     (wmemory_black msc)
       -∗
       (wpoints_to_faa loc v)
       -∗
-      ((⌜(TView.le tvw0 lc2.(Local.tview)) /\ (v = val)⌝)
+      ((⌜(View.le vw0 lc2.(Local.tview).(TView.cur)) /\ (v = val)⌝)
          ∗ #=>((wmemory_black (WMem.mk mem1 sc1)) ∗ wpoints_to_faa loc (Const.add v addendum))).
   Proof.
-  Admitted.
-
+    iIntros "BLACK [% [WHITE %]]". des. subst.
+    iPoseProof (wmemory_ra_get with "BLACK WHITE") as "%". subst.
+    inv READ. inv WRITE. ss.
+    inv WRITE0. ss. hexploit memory_write_bot_add; eauto. i. subst.
+    inv PROMISE. clear REMOVE PROMISES ATTACH TS.
+    hexploit add_succeed_wf; eauto. i. des.
+    assert (MAX0: from = Cell.max_ts (WMem.memory msc loc)).
+    { hexploit FAA; eauto. i. des; auto.
+      hexploit DISJOINT; eauto. i. exfalso. eapply H.
+      { instantiate (1:=Time.meet to to'). econs; ss.
+        { unfold Time.meet. des_ifs. }
+        { eapply Time.meet_l. }
+      }
+      { econs; ss.
+        { unfold Time.meet. des_ifs. }
+        { eapply Time.meet_r. }
+      }
+    }
+    subst. setoid_rewrite GET0 in GET. inv GET.
+    assert (val = v).
+    { inv VAL; ss. destruct val, v; ss. apply Z.eqb_eq in H0. subst. auto. }
+    subst. iSplit.
+    { iPureIntro. split.
+      { etrans; [|eapply View.join_l].
+        etrans; [|eapply View.join_l].
+        eapply View.join_l.
+      }
+      { auto. }
+    }
+    assert (MAX1: to = Cell.max_ts (mem1 loc)).
+    { eapply TimeFacts.antisym.
+      { hexploit Memory.max_ts_spec.
+        { eapply Memory.add_get0; eauto. }
+        { i. des. eauto. }
+      }
+      { hexploit Memory.max_ts_spec.
+        { eapply Memory.add_get1; eauto. }
+        i. des. erewrite Memory.add_o in GET; eauto. des_ifs.
+        { ss. des; subst. reflexivity. }
+        { guardH o. eapply Memory.max_ts_spec in GET. des.
+          etrans ;eauto. left. auto.
+        }
+      }
+    }
+    iPoseProof (wmemory_ra_set with "BLACK WHITE") as "> [BLACK WHITE]".
+    instantiate (1:=mem1 loc). iModIntro. iSplitL "BLACK".
+    { assert (EQ: mem1 = (LocFun.add loc (mem1 loc) (WMem.memory msc))).
+      { inv MEM. extensionality l0. setoid_rewrite LocFun.add_spec. des_ifs.
+        setoid_rewrite LocFun.add_spec_eq. auto.
+      }
+      iEval (rewrite EQ). auto.
+    }
+    iExists _. iSplit; [iFrame|]. iPureIntro. esplits; eauto.
+    { erewrite <- MAX1. eapply Memory.add_get0; eauto. }
+    { i. setoid_rewrite Memory.add_o in GET; [|eauto]. des_ifs.
+      { ss. des; clarify. auto. }
+      { guardH o. hexploit FAA; eauto. i. des.
+        { left. esplits; eauto. eapply Memory.add_get1; eauto. }
+        { subst. left. esplits; eauto.
+          { eapply Memory.add_get0; eauto. }
+        }
+      }
+    }
+    { ii. destruct v, addendum; ss. }
+  Qed.
 
   (* full points-to *)
-  Definition wProp := Const.t -> TView.t -> iProp.
-  Definition wor (P Q: wProp): wProp := fun c vw => ((P c vw) ∨ (Q c vw))%I.
-  Definition wimpl (P Q: wProp): iProp := (∀ c vw, (P c vw) -∗ (Q c vw))%I.
+  Definition wProp := Const.t -> View.t -> Prop.
+  Definition wor (P Q: wProp): wProp := fun c vw => ((P c vw) \/ (Q c vw)).
+  Definition wimpl (P Q: wProp): Prop := (∀ c vw, (P c vw) -> (Q c vw)).
 
-  Definition lift_wProp (P: wProp) (c: Const.t) (vw: TView.t): iProp :=
-    ∃ vw', (P c vw') ∗ (⌜TView.le vw' vw⌝).
+  Definition lift_wProp (P: wProp) (c: Const.t) (vw: View.t): iProp :=
+    ∃ vw', (⌜P c vw'⌝) ∗ (⌜View.le vw' vw⌝).
 
   Lemma lift_wProp_mon
         P c vw0 vw1
-        (LE: TView.le vw0 vw1)
+        (LE: View.le vw0 vw1)
     :
     (lift_wProp P c vw0) -∗ (lift_wProp P c vw1).
   Proof.
@@ -473,92 +448,192 @@ TView.le
   Context `{OBLGRA: @GRA.inG ObligationRA.t Σ}.
   Context `{ARROWRA: @GRA.inG (ArrowRA (void + WMem.ident)%type) Σ}.
 
-  Definition wpoints_to_full (l: Loc.t) (V: TView.t) (k: nat) (P Q: wProp) : iProp.
-  Admitted.
+  Definition wpoints_to_full (l: Loc.t) (V: View.t) (k: nat) (P Q: wProp) : iProp :=
+    ∃ c,
+      (points_to l c)
+        **
+        (∃ v released,
+            (ObligationRA.correl (inr (inr (l, (Cell.max_ts c)))) k (Ord.S Ord.O))
+              **
+              (ObligationRA.pending k 1%Qp)
+              **
+              (⌜Q v View.bot⌝)
+              **
+              (⌜(<<MSGVIEW: V = View.join (View.unwrap released) (View.singleton_ur l (Cell.max_ts c))>>) /\
+                 (<<DEFINED: v <> Const.undef>>) /\
+                 exists from,
+                   (<<GET: Cell.get (Cell.max_ts c) c = Some (from, Message.concrete v released)>>) /\
+                     (<<DEFINED: v <> Const.undef>>) /\
+                     (<<RELEASED: Time.lt Time.bot (Cell.max_ts c) -> released <> None>>)⌝)
+              **
+              (⌜forall to from' v' released' (GET: Cell.get to c = Some (from', Message.concrete v' released'))
+                       (LT: Time.lt to (Cell.max_ts c)),
+                    (P v' View.bot) /\ (<<DEFINED: v' <> Const.undef>>)⌝))
+  .
 
   Lemma wpoints_to_full_not_shot
         l V k P Q
     :
     (wpoints_to_full l V k P Q) ∗ (ObligationRA.shot k) -∗ ⌜False⌝.
   Proof.
-  Admitted.
+    iIntros "[[% [? [% [% [[[[? PENDING] ?] ?] H]]]]] SHOT]".
+    iApply (ObligationRA.pending_not_shot with "PENDING SHOT").
+  Qed.
 
   Lemma wpoints_to_full_impl
         l V k P P' Q
     :
-    ((wimpl P P') ∗ (wpoints_to_full l V k P Q))
+    ((⌜wimpl P P'⌝) ∗ (wpoints_to_full l V k P Q))
       -∗ (wpoints_to_full l V k P' Q).
   Proof.
-  Admitted.
+    iIntros "[% [% [A [% [% [B %]]]]]]".
+    iExists _. iSplitL "A"; [iFrame|]. iExists _, _. iFrame.
+    iIntros (? ? ? ? ? ?). iPureIntro.
+    hexploit H0; eauto. i. des. split; auto.
+  Qed.
 
   Lemma wmemory_ra_load_acq
         l V k (P Q: wProp)
         m val vw0 vw1
         ord lc1 to released
-        (READ: Local.read_step (Local.mk vw0 Memory.bot) m.(WMem.memory) l to val released ord lc1)
-        (VIEW: vw1 = lc1.(Local.tview))
+        (READ: Local.read_step (WMem.view_to_local vw0) m.(WMem.memory) l to val released ord lc1)
+        (VIEW: vw1 = lc1.(Local.tview).(TView.cur))
         (ORD: ord = Ordering.acqrel)
     :
     (wmemory_black m)
       -∗
       (wpoints_to_full l V k P Q)
       -∗
-      ((⌜TView.le vw0 vw1⌝)
+      ((⌜View.le vw0 vw1⌝)
          ∗ (wmemory_black m)
          ∗ (wpoints_to_full l V k P Q)
          ∗ (((lift_wProp P val vw1)
                ∗ (∃ ts, (ObligationRA.correl (inr (inr (l, ts))) k (Ord.S Ord.O))
                           ∗ (⌜WMem.missed m.(WMem.memory) l to (l, ts) = Flag.fail⌝)))
-            ∨ ((lift_wProp Q val vw1) ∗ (⌜TView.le V vw1⌝)))
+            ∨ ((lift_wProp Q val vw1) ∗ (⌜View.le V vw1⌝)))
       ).
   Proof.
-  Admitted.
+    iIntros "BLACK [% [WHITE [% [% [[[[#X Y] %] %] %]]]]]". des. subst.
+    iPoseProof (wmemory_ra_get with "BLACK WHITE") as "%". subst.
+    inv READ. ss. iSplit.
+    { iPureIntro. aggrtac. }
+    iSplitL "BLACK"; [auto|]. iSplitL.
+    { iExists _. iFrame. iExists _, _. iSplit.
+      { iSplit.
+        { iSplit; auto. }
+        { iPureIntro. esplits; eauto. }
+      }
+      { iPureIntro. auto. }
+    }
+    destruct (Time.eq_dec to (Cell.max_ts (WMem.memory m l))).
+    { iRight. subst. setoid_rewrite GET0 in GET. inv GET.
+      assert (val = v).
+      { inv VAL; ss.
+        destruct v, val; ss. apply Z.eqb_eq in H2. subst. auto.
+      }
+      subst. iSplit.
+      { unfold lift_wProp. iExists _. iSplit.
+        { iPureIntro. eauto. }
+        { iPureIntro. apply View.bot_spec. }
+      }
+      { iPureIntro. unfold View.singleton_ur_if. des_ifs.
+        eapply View.join_spec.
+        { aggrtac. }
+        { etrans; [|eapply View.join_l]. eapply View.join_r. }
+      }
+    }
+    { iLeft. hexploit Memory.max_ts_spec.
+      { eapply GET0. }
+      i. des. dup MAX. inv MAX; ss.
+      hexploit H1; eauto. i. des.
+      assert (val' = val).
+      { inv VAL; ss. destruct val, val'; ss. apply Z.eqb_eq in H4. subst. auto. }
+      subst. iSplitR.
+      { unfold lift_wProp. iExists _. iSplit.
+        { iPureIntro. eapply H1; eauto. }
+        { iPureIntro. apply View.bot_spec. }
+      }
+      iExists _. iSplitR; auto. iPureIntro.
+      destruct (LocSet.Facts.eq_dec l l); ss.
+      destruct (Time.le_lt_dec (Cell.max_ts (WMem.memory m l)) to).
+      { exfalso. eapply Time.lt_strorder.
+        eapply TimeFacts.lt_le_lt; [|apply l0]; eauto.
+      }
+      setoid_rewrite GET. hexploit RELEASED; auto.
+      { eapply TimeFacts.le_lt_lt; eauto. eapply Time.bot_spec. }
+      { i. des_ifs. }
+    }
+  Qed.
 
   Lemma wmemory_ra_load_rlx
         l V k (P Q: wProp)
         m val vw0 vw1
         ord lc1 to released
-        (READ: Local.read_step (Local.mk vw0 Memory.bot) m.(WMem.memory) l to val released ord lc1)
-        (VIEW: vw1 = lc1.(Local.tview))
+        (READ: Local.read_step (WMem.view_to_local vw0) m.(WMem.memory) l to val released ord lc1)
+        (VIEW: vw1 = lc1.(Local.tview).(TView.cur))
         (ORD: ord = Ordering.relaxed)
     :
     (wmemory_black m)
       -∗
       (wpoints_to_full l V k P Q)
       -∗
-      (⌜TView.le V vw0⌝)
+      (⌜View.le V vw0⌝)
       -∗
-      ((⌜TView.le vw0 vw1⌝)
+      ((⌜View.le vw0 vw1⌝)
          ∗ (wmemory_black m)
          ∗ (wpoints_to_full l V k P Q)
          ∗ (lift_wProp Q val vw1)
       ).
   Proof.
-  Admitted.
+    iIntros "BLACK [% [WHITE [% [% [[[X %] %] Z]]]]] %". des. subst.
+    iPoseProof (wmemory_ra_get with "BLACK WHITE") as "%". subst.
+    inv READ. ss.
+    assert (TO: to = Cell.max_ts (WMem.memory m l)).
+    { eapply TimeFacts.antisym.
+      { eapply Memory.max_ts_spec in GET0. des. clarify. }
+      { inv READABLE. etrans; eauto.
+        inv H1. ss. specialize (PLN0 l).
+        unfold TimeMap.singleton in PLN0. etrans; [|eauto].
+        unfold TimeMap.join. setoid_rewrite LocFun.add_spec_eq.
+        apply Time.join_r.
+      }
+    }
+    subst. setoid_rewrite GET0 in GET. inv GET.
+    assert (val = v).
+    { inv VAL; ss.
+      destruct v, val; ss. apply Z.eqb_eq in H2. subst. auto.
+    }
+    subst. iSplit.
+    { iPureIntro. aggrtac. }
+    iSplitL "BLACK"; [auto|]. iSplitL.
+    { iExists _. iFrame. iExists _, _. iSplit; eauto. iPureIntro. esplits; eauto. }
+    { unfold lift_wProp. iExists _. iPureIntro. splits; eauto. eapply View.bot_spec. }
+  Qed.
 
   Lemma wmemory_ra_store_rel
         l V k (P Q R: wProp)
         m0 vw0 m1 val vw1
         lc1 to sc1 mem1 ord from released kind
-        (WRITE: Local.write_step (Local.mk vw0 Memory.bot) m0.(WMem.sc) m0.(WMem.memory) l from to val None released ord lc1 sc1 mem1 kind)
-        (VIEW: vw1 = lc1.(Local.tview))
+        (WRITE: Local.write_step (WMem.view_to_local vw0) m0.(WMem.sc) m0.(WMem.memory) l from to val None released ord lc1 sc1 mem1 kind)
+        (VIEW: vw1 = lc1.(Local.tview).(TView.cur))
         (MEM: m1 = WMem.mk mem1 sc1)
         (ORD: ord = Ordering.acqrel)
+        (DEFINED: val <> Const.undef)
     :
     (wmemory_black m0)
       -∗
       (wpoints_to_full l V k P Q)
       -∗
-      (⌜TView.le V vw0⌝)
+      (⌜View.le V vw0⌝)
       -∗
-      (R val vw0)
+      (⌜R val vw0⌝)
       -∗
-      ((⌜TView.le vw0 vw1⌝)
+      ((⌜View.le vw0 vw1⌝)
          ∗ #=>((wmemory_black m1))
          ∗ (∃ V' k' o,
-               (⌜TView.le V' vw1⌝)
+               (⌜View.le V' vw1⌝)
                  ∗
-                 (⌜TView.le vw0 V'⌝)
+                 (⌜View.le vw0 V'⌝)
                  ∗
                  #=>((wpoints_to_full l V' k' (wor P Q) R)
                        ∗ (ObligationRA.black k' o)
@@ -566,6 +641,91 @@ TView.le
            )
       ).
   Proof.
+    iIntros "BLACK [% [WHITE [% [% [[[[#X Y] %] %] %]]]]] % %". des. subst.
+    iPoseProof (wmemory_ra_get with "BLACK WHITE") as "%". subst.
+    inv WRITE. ss. iSplit.
+    { iPureIntro. aggrtac. }
+    hexploit memory_write_bot_add; eauto. i. subst.
+    inv WRITE0. inv PROMISE. clear REMOVE PROMISES ATTACH TS.
+    iPoseProof (wmemory_ra_set with "BLACK WHITE") as "> [BLACK WHITE]".
+    instantiate (1:=mem1 l). iModIntro. iSplitL "BLACK".
+    { assert (EQ: mem1 = (LocFun.add l (mem1 l) (WMem.memory m0))).
+      { inv MEM. extensionality l0. setoid_rewrite LocFun.add_spec. des_ifs.
+        setoid_rewrite LocFun.add_spec_eq. auto.
+      }
+      iEval (rewrite EQ). auto.
+    }
+
+
+    iExists _,
+    assert (MAX: Cell.max_ts (mem1 l) = to).
+    { hexploit Memory.max_ts_spec.
+      { eapply Memory.add_get1; eauto. }
+      i. des. erewrite Memory.add_o in GET0; eauto. des_ifs; ss.
+      { des; clarify. }
+      { des; ss. eapply Memory.max_ts_spec in GET0. des.
+        hexploit Memory.max_ts_spec.
+        { eapply Memory.add_get0; eauto. }
+        i. des. inv WRITABLE.
+        exfalso. eapply Time.lt_strorder. eapply TimeFacts.lt_le_lt.
+        { eapply TS. }
+        etrans; eauto.
+        etrans; eauto.
+        inv VIEW0. ss. specialize (RLX l).
+        unfold TimeMap.singleton in RLX. setoid_rewrite LocFun.add_spec_eq in RLX. auto.
+      }
+    }
+
+
+    iSplitL "BLACK"; [auto|]. iSplitL.
+    { iExists _. iFrame. iExists _, _. iSplit.
+      { iSplit.
+        { iSplit; auto. }
+        { iPureIntro. esplits; eauto. }
+      }
+      { iPureIntro. auto. }
+    }
+    destruct (Time.eq_dec to (Cell.max_ts (WMem.memory m l))).
+    { iRight. subst. setoid_rewrite GET0 in GET. inv GET.
+      assert (val = v).
+      { inv VAL; ss.
+        destruct v, val; ss. apply Z.eqb_eq in H2. subst. auto.
+      }
+      subst. iSplit.
+      { unfold lift_wProp. iExists _. iSplit.
+        { iPureIntro. eauto. }
+        { iPureIntro. apply View.bot_spec. }
+      }
+      { iPureIntro. unfold View.singleton_ur_if. des_ifs.
+        eapply View.join_spec.
+        { aggrtac. }
+        { etrans; [|eapply View.join_l]. eapply View.join_r. }
+      }
+    }
+    { iLeft. hexploit Memory.max_ts_spec.
+      { eapply GET0. }
+      i. des. dup MAX. inv MAX; ss.
+      hexploit H1; eauto. i. des.
+      assert (val' = val).
+      { inv VAL; ss. destruct val, val'; ss. apply Z.eqb_eq in H4. subst. auto. }
+      subst. iSplitR.
+      { unfold lift_wProp. iExists _. iSplit.
+        { iPureIntro. eapply H1; eauto. }
+        { iPureIntro. apply View.bot_spec. }
+      }
+      iExists _. iSplitR; auto. iPureIntro.
+      destruct (LocSet.Facts.eq_dec l l); ss.
+      destruct (Time.le_lt_dec (Cell.max_ts (WMem.memory m l)) to).
+      { exfalso. eapply Time.lt_strorder.
+        eapply TimeFacts.lt_le_lt; [|apply l0]; eauto.
+      }
+      setoid_rewrite GET. hexploit RELEASED; auto.
+      { eapply TimeFacts.le_lt_lt; eauto. eapply Time.bot_spec. }
+      { i. des_ifs. }
+    }
+  Qed.
+
+
   Admitted.
 
 End MEMRA.
